Add semantics for some control-flow and synchronization operators

isa.dfy
@@ -4,32 +4,39 @@ type PEIndex = int
 type Value = int
 
 datatype CarryState = CarryI | CarryB1 | CarryB2
+datatype MergeState = MergeI | MergeA | MergeB
 
 datatype ProcessingElement =
-    AddOperator       (                   a: ChannelIndex, b: ChannelIndex,                 outputs: seq<ChannelIndex>)
-    // AccMuliplyOperator(acc: Value,        d: ChannelIndex, a: ChannelIndex,                 outputs: seq<ChannelIndex>) |
-    // CarryOperator     (state: CarryState, d: ChannelIndex, a: ChannelIndex, b: ChannelIndex, outputs: seq<ChannelIndex>) |
-    // TrueSteerOperator (a: ChannelIndex, d: ChannelIndex,                 outputs: seq<ChannelIndex>) |
-    // SelectOperator    (d: ChannelIndex, a: ChannelIndex, b: ChannelIndex, outputs: seq<ChannelIndex>) |
-    // OrderOperator     (a: ChannelIndex, b: ChannelIndex,                 outputs: seq<ChannelIndex>) |
-    // MergeOperator     (                   d: ChannelIndex, a: ChannelIndex, b: ChannelIndex, outputs: seq<ChannelIndex>)
+    AddOperator       (                        a: ChannelIndex, b: ChannelIndex,                  outputs: seq<ChannelIndex>) |
+    CarryOperator     (carryState: CarryState, d: ChannelIndex, a: ChannelIndex, b: ChannelIndex, outputs: seq<ChannelIndex>) |
+    TrueSteerOperator (                        d: ChannelIndex, a: ChannelIndex,                  outputs: seq<ChannelIndex>) |
+    FalseSteerOperator(                        d: ChannelIndex, a: ChannelIndex,                  outputs: seq<ChannelIndex>) |
+    SelectOperator    (                        d: ChannelIndex, a: ChannelIndex, b: ChannelIndex, outputs: seq<ChannelIndex>) |
+    OrderOperator     (                        a: ChannelIndex, b: ChannelIndex,                  outputs: seq<ChannelIndex>) |
+    MergeOperator     (mergeState: MergeState, d: ChannelIndex, a: ChannelIndex, b: ChannelIndex, outputs: seq<ChannelIndex>)
 {
     // Get all input channel indices of a PE
     function method Inputs(): seq<ChannelIndex> {
         match this
-            case AddOperator(a, b, outputs) => [a, b]
-            // case AccMuliplyOperator(acc, d, a, outputs) => [d, a]
-            // case CarryOperator(state, d, a, b, outputs) => [d, a, b]
-            // case MergeOperator(d, a, b, outputs) => [d, a, b]
+            case AddOperator(a, b, _) => [a, b]
+            case CarryOperator(_, d, a, b, _) => [d, a, b]
+            case TrueSteerOperator(d, a, _) => [d, a]
+            case FalseSteerOperator(d, a, _) => [d, a]
+            case SelectOperator(d, a, b, _) => [d, a, b]
+            case OrderOperator(a, b, _) => [a, b]
+            case MergeOperator(_, d, a, b, _) => [d, a, b]
     }
 
     // Get all output channel indices of a PE
     function method Outputs(): seq<ChannelIndex> {
         match this
-            case AddOperator(a, b, outputs) => outputs
-            // case AccMuliplyOperator(acc, d, a, outputs) => outputs
-            // case CarryOperator(state, d, a, b, outputs) => outputs
-            // case MergeOperator(d, a, b, outputs) => outputs
+            case AddOperator(_, _, outputs) => outputs
+            case CarryOperator(_, _, _, _, outputs) => outputs
+            case TrueSteerOperator(_, _, outputs) => outputs
+            case FalseSteerOperator(_, _, outputs) => outputs
+            case SelectOperator(_, _, _, outputs) => outputs
+            case OrderOperator(_, _, output) => outputs
+            case MergeOperator(_, _, _, _, outputs) => outputs
     }
 
     // Get the input channel indices a PE is currently waiting on
@@ -37,15 +44,23 @@ datatype ProcessingElement =
         ensures multiset(WaitingInputs()) <= multiset(Inputs())
     {
         match this {
-            case AddOperator(a, b, outputs) => [a, b]
-            // case AccMuliplyOperator(acc, d, a, outputs) => [d, a]
-            // case CarryOperator(state, d, a, b, outputs) =>
-            //     match state {
-            //         case CarryI => [a]
-            //         case CarryB1 => [d]
-            //         case CarryB2 => [b]
-            //     }
-            // case MergeOperator(d, a, b, outputs) => [d, a, b]
+            case AddOperator(a, b, _) => [a, b]
+            case CarryOperator(state, d, a, b, _) =>
+                match state {
+                    case CarryI => [a]
+                    case CarryB1 => [d]
+                    case CarryB2 => [b]
+                }
+            case TrueSteerOperator(d, a, _) => [d, a]
+            case FalseSteerOperator(d, a, _) => [d, a]
+            case SelectOperator(d, a, b, _) => [d, a, b]
+            case OrderOperator(a, b, _) => [a, b]
+            case MergeOperator(state, d, a, b, _) =>
+                match state {
+                    case MergeI => [d]
+                    case MergeA => [a]
+                    case MergeB => [b]
+                }
         }
     }
 }
@@ -113,6 +128,7 @@ datatype DataflowProgramState = DataflowProgramState(channels: seq<Channel>, pro
         requires 0 <= idx < |processingElements|
     {
         forall ChannelIndex :: ChannelIndex in processingElements[idx].WaitingInputs() ==>
+            ChannelIndex in processingElements[idx].Inputs() && // TODO: this is not necessary
             channels[ChannelIndex].Length() != 0
     }
 
@@ -160,7 +176,7 @@ datatype DataflowProgramState = DataflowProgramState(channels: seq<Channel>, pro
         var pe := processingElements[idx];
         match pe
             case AddOperator(a, b, outputs) =>
-                assert a in pe.WaitingInputs() && b in pe.WaitingInputs();
+                assert a in pe.Inputs() && b in pe.Inputs();
                 assert outputs <= pe.Outputs();
                 // assert a == pe.Inputs()[0] && b == pe.Inputs()[1];
                 // assert a != b;
@@ -171,6 +187,135 @@ datatype DataflowProgramState = DataflowProgramState(channels: seq<Channel>, pro
                 var newState := DataflowProgramState(newChannels, processingElements);
 
                 newState.Multicast(valA + valB, outputs)
+
+            case TrueSteerOperator(d, a, outputs) =>
+                assert d in pe.Inputs() && a in pe.Inputs();
+                assert outputs <= pe.Outputs();
+
+                var (valD, newChannelD) := channels[d].Receive();
+                var (valA, newChannelA) := channels[a].Receive();
+                var newChannels := channels[d := newChannelD][a := newChannelA];
+                var newState := DataflowProgramState(newChannels, processingElements);
+
+                if valD == 1 then
+                    newState.Multicast(valA , outputs)
+                else
+                    newState
+
+            case FalseSteerOperator(d, a, outputs) =>
+                assert d in pe.Inputs() && a in pe.Inputs();
+                assert outputs <= pe.Outputs();
+
+                var (valD, newChannelD) := channels[d].Receive();
+                var (valA, newChannelA) := channels[a].Receive();
+                var newChannels := channels[d := newChannelD][a := newChannelA];
+                var newState := DataflowProgramState(newChannels, processingElements);
+
+                if valD == 0 then
+                    newState.Multicast(valA , outputs)
+                else
+                    newState
+            
+            case SelectOperator(d, a, b, outputs) =>
+                assert d in pe.Inputs() && a in pe.Inputs() && b in pe.Inputs();
+                assert outputs <= pe.Outputs();
+
+                var (valD, newChannelD) := channels[d].Receive();
+                var (valA, newChannelA) := channels[a].Receive();
+                var (valB, newChannelB) := channels[b].Receive();
+                var newChannels := channels[d := newChannelD][a := newChannelA][b := newChannelB];
+                var newState := DataflowProgramState(newChannels, processingElements);
+
+                if valD == 1 then
+                    newState.Multicast(valA, outputs)
+                else
+                    newState.Multicast(valB, outputs)
+
+            case CarryOperator(state, d, a, b, outputs) =>
+                match state {
+                    case CarryI =>
+                        assert a in pe.Inputs();
+
+                        var (valA, newChannelA) := channels[a].Receive();
+                        var newChannels := channels[a := newChannelA];
+                        var newPEs := processingElements[idx := CarryOperator(CarryB1, d, a, b, outputs)];
+                        var newState := DataflowProgramState(newChannels, newPEs);
+
+                        assert forall i :: 0 <= i < |newPEs| ==> newPEs[i].Inputs() == processingElements[i].Inputs();
+                        newState.Multicast(valA, outputs)
+
+                    case CarryB1 =>
+                        assert d in pe.Inputs();
+
+                        var (valD, newChannelD) := channels[d].Receive();
+                        var newChannels := channels[d := newChannelD];
+
+                        var updatedPE := if valD == 0 then CarryOperator(CarryI, d, a, b, outputs)
+                                                      else CarryOperator(CarryB2, d, a, b, outputs);
+                        var newPEs := processingElements[idx := updatedPE];
+
+                        DataflowProgramState(newChannels, newPEs)
+                        
+                    case CarryB2 =>
+                        assert b in pe.Inputs();
+
+                        var (valB, newChannelB) := channels[b].Receive();
+                        var newChannels := channels[b := newChannelB];
+                        var newPEs := processingElements[idx := CarryOperator(CarryB1, d, a, b, outputs)];
+                        var newState := DataflowProgramState(newChannels, newPEs);
+
+                        assert forall i :: 0 <= i < |newPEs| ==> newPEs[i].Inputs() == processingElements[i].Inputs();
+                        newState.Multicast(valB, outputs)
+                }
+
+            case OrderOperator(a, b, outputs) =>
+                assert a in pe.Inputs() && b in pe.Inputs();
+                assert outputs <= pe.Outputs();
+                
+                var (valA, newChannelA) := channels[a].Receive();
+                var (valB, newChannelB) := channels[b].Receive();
+                var newChannels := channels[a := newChannelA][b := newChannelB];
+                var newState := DataflowProgramState(newChannels, processingElements);
+
+                newState.Multicast(valB, outputs)
+
+            case MergeOperator(state, d, a, b, outputs) =>
+                match state {
+                    case MergeI =>
+                        assert d in pe.Inputs();
+
+                        var (valD, newChannelD) := channels[d].Receive();
+                        var newChannels := channels[d := newChannelD];
+
+                        var updatedPE := if valD == 0 then MergeOperator(MergeA, d, a, b, outputs)
+                                                      else MergeOperator(MergeB, d, a, b, outputs);
+                        var newPEs := processingElements[idx := updatedPE];
+
+                        DataflowProgramState(newChannels, newPEs)
+
+                    case MergeA =>
+                        assert a in pe.Inputs();
+
+                        var (valA, newChannelA) := channels[a].Receive();
+                        var newChannels := channels[a := newChannelA];
+                        var newPEs := processingElements[idx := MergeOperator(MergeI, d, a, b, outputs)];
+                        var newState := DataflowProgramState(newChannels, newPEs);
+
+                        assert forall i :: 0 <= i < |newPEs| ==> newPEs[i].Inputs() == processingElements[i].Inputs();
+                        newState.Multicast(valA, outputs)
+
+                    case MergeB =>
+                        assert b in pe.Inputs();
+
+                        var (valB, newChannelB) := channels[b].Receive();
+                        var newChannels := channels[b := newChannelB];
+                        var newPEs := processingElements[idx := MergeOperator(MergeI, d, a, b, outputs)];
+                        var newState := DataflowProgramState(newChannels, newPEs);
+
+                        assert forall i :: 0 <= i < |newPEs| ==> newPEs[i].Inputs() == processingElements[i].Inputs();
+                        newState.Multicast(valB, outputs)
+                }
+
     }
 
     predicate AreBothFireable(idx1: PEIndex, idx2: PEIndex)
@@ -186,8 +331,16 @@ datatype DataflowProgramState = DataflowProgramState(channels: seq<Channel>, pro
         requires AreBothFireable(idx1, idx2)
         requires idx1 != idx2
         ensures FirePE(idx1).IsFireable(idx2)
-    {}
+    {
+        // match (processingElements[idx1], processingElements[idx2]) {
+        //     case (AddOperator(_, _, _), AddOperator(_, _, _)) => {}
+        //     case (AddOperator(_, _, _), CarryOperator(_, _, _, _, _)) => {}
+        //     case (CarryOperator(_, _, _, _, _), AddOperator(_, _, _)) => {}
+        //     case (CarryOperator(_, _, _, _, _), CarryOperator(_, _, _, _, _)) => {}
+        // }
+    }
 
+    // This might need longer timeouts
     lemma FirePEConfluence(idx1: PEIndex, idx2: PEIndex)
         requires Wellformed()
         requires AreBothFireable(idx1, idx2)
