Makefile
@@ -1,0 +1,3 @@
+.PHONY: verify
+verify:
+	dafny /compile:0 /timeLimit:600 isa.dfy
